prove prevLog leader sublog

raft-proofs/PrevLogLeaderSublogProof.v
@@ -11,16 +11,403 @@ Require Import Net.
 Require Import Raft.
 Require Import VerdiTactics.
 Require Import CommonTheorems.
+Require Import SpecLemmas.
+Require Import RaftRefinementInterface.
+
+Require Import PrevLogCandidateEntriesTermInterface.
+Require Import VotesCorrectInterface.
+Require Import CroniesCorrectInterface.
+Require Import LeaderSublogInterface.
 
 Require Import PrevLogLeaderSublogInterface.
+
+Hint Extern 4 (@BaseParams) => apply base_params : typeclass_instances.
+Hint Extern 4 (@MultiParams _) => apply multi_params : typeclass_instances.
+Hint Extern 4 (@FailureParams _ _) => apply failure_params : typeclass_instances.
+
 
 Section PrevLogLeaderSublogProof.
   Context {orig_base_params : BaseParams}.
   Context {one_node_params : OneNodeParams orig_base_params}.
   Context {raft_params : RaftParams orig_base_params}.
 
+  Context {rri : raft_refinement_interface}.
+
+  Context {vci : votes_correct_interface}.
+  Context {cci : cronies_correct_interface}.
+
+  Context {lsi : leader_sublog_interface}.
+
+  Context {plceti : prevLog_candidateEntriesTerm_interface}.
+
+  Lemma prevLog_leader_sublog_init :
+   raft_net_invariant_init prevLog_leader_sublog.
+  Proof.
+    unfold raft_net_invariant_init, prevLog_leader_sublog.
+    simpl. intuition.
+  Qed.
+
+  Lemma handleClientRequest_log_In :
+    forall h st client id c out st' ps e,
+      handleClientRequest h st client id c = (out, st', ps) ->
+      In e (log st) -> In e (log st').
+  Proof.
+    intros.
+    find_apply_lem_hyp handleClientRequest_log.
+    intuition.
+    - find_rewrite. auto.
+    - break_exists. intuition. find_rewrite. intuition.
+  Qed.
+
+  Lemma prevLog_leader_sublog_client_request :
+    raft_net_invariant_client_request prevLog_leader_sublog.
+  Proof.
+    unfold raft_net_invariant_client_request, prevLog_leader_sublog.
+    intros. simpl in *.
+    repeat find_higher_order_rewrite.
+    find_apply_hyp_hyp. break_or_hyp.
+    - break_if; eauto.
+      find_copy_apply_lem_hyp handleClientRequest_type. break_and.
+      repeat find_rewrite.
+      eapply_prop_hyp In In; eauto.
+      break_exists_exists. intuition.
+      eauto using handleClientRequest_log_In.
+    - find_apply_lem_hyp in_map_iff. break_exists. break_and.
+      exfalso. eapply handleClientRequest_no_append_entries; eauto.
+      subst. simpl in *. find_rewrite. eauto 10.
+  Qed.
+
+  Lemma prevLog_leader_sublog_timeout :
+    raft_net_invariant_timeout prevLog_leader_sublog.
+  Proof.
+    unfold raft_net_invariant_timeout, prevLog_leader_sublog.
+    intros. simpl in *.
+    repeat find_higher_order_rewrite.
+    find_apply_hyp_hyp. break_or_hyp.
+    - break_if; eauto.
+      find_copy_apply_lem_hyp handleTimeout_type.
+      intuition; repeat find_rewrite; try discriminate.
+      eapply_prop_hyp In In; eauto.
+      break_exists_exists. intuition.
+      erewrite handleTimeout_log_same by eauto.
+      eauto.
+    - find_apply_lem_hyp in_map_iff. break_exists. break_and.
+      exfalso. subst. simpl in *.
+      eapply handleTimeout_packets; eauto.
+      find_rewrite. eauto 10.
+  Qed.
+
+  Lemma handleAppendEntries_type_log :
+    forall h st t n pli plt es ci st' ps,
+      handleAppendEntries h st t n pli plt es ci = (st', ps) ->
+      type st' = Follower \/ (type st' = type st /\ log st' = log st /\ currentTerm st' = currentTerm st).
+  Proof.
+    unfold handleAppendEntries.
+    intros.
+    repeat break_match; repeat find_inversion; simpl in *; auto.
+  Qed.
+
+  Lemma prevLog_leader_sublog_append_entries :
+    raft_net_invariant_append_entries prevLog_leader_sublog.
+  Proof.
+    unfold raft_net_invariant_append_entries, prevLog_leader_sublog.
+    intros. simpl in *.
+    repeat find_higher_order_rewrite.
+    find_apply_hyp_hyp. break_or_hyp.
+    - find_eapply_lem_hyp app_cons_in_rest; [|solve[eauto]].
+      find_rewrite. break_if; eauto.
+      find_copy_apply_lem_hyp handleAppendEntries_type_log.
+      intuition.
+      + congruence.
+      + repeat find_rewrite.
+        eapply_prop_hyp In In; eauto.
+    - find_apply_lem_hyp handleAppendEntries_not_append_entries.
+      simpl in *. subst. exfalso. eauto 10.
+  Qed.
+
+  Lemma prevLog_leader_sublog_append_entries_reply :
+    raft_net_invariant_append_entries_reply prevLog_leader_sublog.
+  Proof.
+    unfold raft_net_invariant_append_entries_reply, prevLog_leader_sublog.
+    intros. simpl in *.
+    repeat find_higher_order_rewrite.
+    find_apply_hyp_hyp. break_or_hyp.
+    - find_eapply_lem_hyp app_cons_in_rest; [|solve[eauto]].
+      find_rewrite. break_if; eauto.
+      find_copy_apply_lem_hyp handleAppendEntriesReply_log.
+      find_rewrite.
+      find_copy_apply_lem_hyp handleAppendEntriesReply_type.
+      intuition; repeat find_rewrite; try discriminate.
+      eauto.
+    - find_apply_lem_hyp in_map_iff. break_exists. break_and.
+      exfalso. subst. simpl in *.
+      find_apply_lem_hyp handleAppendEntriesReply_packets.
+      subst. simpl in *. intuition.
+  Qed.
+
+  Lemma prevLog_leader_sublog_request_vote :
+    raft_net_invariant_request_vote prevLog_leader_sublog.
+  Proof.
+    unfold raft_net_invariant_request_vote, prevLog_leader_sublog.
+    intros. simpl in *.
+    repeat find_higher_order_rewrite.
+    find_apply_hyp_hyp. break_or_hyp.
+    - find_eapply_lem_hyp app_cons_in_rest; [|solve[eauto]].
+      find_rewrite. break_if; eauto.
+      find_copy_apply_lem_hyp handleRequestVote_log.
+      find_copy_apply_lem_hyp handleRequestVote_type.
+      intuition; repeat find_rewrite; try discriminate.
+      eauto.
+    - find_apply_lem_hyp handleRequestVote_no_append_entries.
+      simpl in *. subst. exfalso. eauto 10.
+  Qed.
+
+
+  Definition candidateEntriesTerm_lowered (net : network) t p : Prop :=
+    In p (nwPackets net) ->
+    pBody p = RequestVoteReply t true ->
+    currentTerm (nwState net (pDst p)) = t ->
+    wonElection (dedup name_eq_dec (pSrc p :: votesReceived (nwState net (pDst p)))) = true ->
+    type (nwState net (pDst p)) <> Candidate.
+
+  Lemma deghost_packet_exists :
+    forall net p,
+      In p (nwPackets (deghost net)) ->
+      exists (q : packet (params := raft_refined_multi_params (raft_params := raft_params))),
+        In q (nwPackets net) /\ p = deghost_packet q.
+  Proof.
+    unfold deghost.
+    simpl.
+    intros.
+    do_in_map.
+    eauto.
+  Qed.
+
+  Lemma prevLog_candidateEntriesTerm_lowered' :
+    forall net,
+      prevLog_candidateEntriesTerm net ->
+      votes_correct net ->
+      cronies_correct net ->
+      forall p p' t leaderId prevLogIndex prevLogTerm entries leaderCommit,
+        In p (nwPackets (deghost net)) ->
+        pBody p = AppendEntries t leaderId prevLogIndex prevLogTerm
+                                entries leaderCommit ->
+        candidateEntriesTerm_lowered (deghost net) prevLogTerm p'.
+  Proof.
+    unfold candidateEntriesTerm_lowered,
+           cronies_correct, votes_correct.
+    intros. break_and.
+    rewrite deghost_spec.
+
+    find_apply_lem_hyp deghost_packet_exists.
+    find_apply_lem_hyp deghost_packet_exists.
+    break_exists.  break_and. subst.
+    eapply_prop_hyp votes_nw pBody. concludes.
+    eapply_prop_hyp prevLog_candidateEntriesTerm pBody; auto.
+
+    unfold candidateEntriesTerm in *. break_exists. break_and.
+
+    match goal with
+    | H : wonElection _ = _ |- _ =>
+      eapply wonElection_one_in_common in H; [|clear H; eauto]
+    end.
+    break_exists. break_and.
+    repeat match goal with
+           | [ H : _ |- _ ] => rewrite deghost_spec in H
+           end.
+
+    simpl in *.
+    break_or_hyp.
+    - apply_prop_hyp cronies_votes In.
+      assert (pDst x = x1) by (eapply_prop one_vote_per_term; eauto).
+      subst. auto.
+    - intro.
+      assert (pDst x = x1).
+      { eapply_prop one_vote_per_term;
+        eapply_prop cronies_votes.
+        - eapply_prop votes_received_cronies; eauto.
+        - repeat find_reverse_rewrite. auto.
+      }
+      subst.
+      concludes. contradiction.
+  Qed.
+
+  Lemma prevLog_candidateEntriesTerm_lowered :
+    forall net,
+      raft_intermediate_reachable net ->
+      forall p p' t leaderId prevLogIndex prevLogTerm entries leaderCommit,
+        In p (nwPackets net) ->
+        pBody p = AppendEntries t leaderId prevLogIndex prevLogTerm
+                                entries leaderCommit ->
+        candidateEntriesTerm_lowered net prevLogTerm p'.
+  Proof.
+    intros net H.
+    pattern net.
+    apply lower_prop; auto.
+    clear H net.
+    intros.
+
+    eapply prevLog_candidateEntriesTerm_lowered';
+      eauto using prevLog_candidateEntriesTerm_invariant, votes_correct_invariant,
+      cronies_correct_invariant.
+  Qed.
+
+  Lemma handleRequestVoteReply_type_term_won :
+    forall h st src t v st',
+      handleRequestVoteReply h st src t v = st' ->
+      type st' = type st \/
+      type st' = Follower \/
+      (v = true /\
+       wonElection (dedup name_eq_dec (src :: votesReceived st)) = true /\
+       currentTerm st' = t).
+  Proof.
+    unfold handleRequestVoteReply.
+    intros.
+    repeat break_match; repeat find_inversion; subst; simpl in *; auto; do_bool; intuition.
+  Qed.
+
+  Lemma prevLog_leader_sublog_request_vote_reply :
+    raft_net_invariant_request_vote_reply prevLog_leader_sublog.
+  Proof.
+    unfold raft_net_invariant_request_vote_reply, prevLog_leader_sublog.
+    intros. simpl in *.
+    repeat find_higher_order_rewrite.
+    find_apply_hyp_hyp.
+    find_eapply_lem_hyp app_cons_in_rest; [|solve[eauto]].
+    find_rewrite. break_if; eauto.
+    find_copy_apply_lem_hyp handleRequestVoteReply_type.
+    find_copy_apply_lem_hyp handleRequestVoteReply_log.
+    intuition; repeat find_rewrite.
+    - eauto.
+    - discriminate.
+    - exfalso.
+      find_apply_lem_hyp handleRequestVoteReply_type_term_won.
+      intuition; try congruence.
+      eapply prevLog_candidateEntriesTerm_lowered with (p := p0) ; eauto.
+      + congruence.
+      + congruence.
+  Qed.
+
+  Lemma doLeader_messages :
+    forall st h os st' ms m t n pli plt es ci,
+      doLeader st h = (os, st', ms) ->
+      In m ms ->
+      snd m = AppendEntries t n pli plt es ci ->
+      t = currentTerm st /\
+      log st' = log st /\
+      type st = Leader /\
+      ((plt = 0) \/
+       ((exists e, findAtIndex (log st) pli = Some e /\
+              eTerm e = plt))).
+  Proof.
+    intros. unfold doLeader, advanceCommitIndex in *.
+    break_match; try solve [find_inversion; simpl in *; intuition].
+    break_if; try solve [find_inversion; simpl in *; intuition].
+    find_inversion. simpl. do_in_map. subst.
+    simpl in *. find_inversion. intuition.
+    match goal with
+      | |- context [pred ?x] =>
+        remember (pred x) as index
+    end. break_match; simpl in *.
+    - right. eauto.
+    - destruct index; intuition.
+  Qed.
+
+  Lemma prevLog_leader_sublog_do_leader :
+    raft_net_invariant_do_leader prevLog_leader_sublog.
+  Proof.
+    unfold raft_net_invariant_do_leader, prevLog_leader_sublog.
+    intros. simpl in *.
+    repeat find_higher_order_rewrite.
+    find_apply_hyp_hyp. break_or_hyp.
+    - break_if; eauto.
+      find_copy_apply_lem_hyp doLeader_type. break_and.
+      find_copy_apply_lem_hyp doLeader_log.
+      repeat find_rewrite. eauto.
+    - find_apply_lem_hyp in_map_iff. break_exists. break_and. subst.
+      simpl in *.
+      find_copy_eapply_lem_hyp doLeader_messages; eauto.
+      intuition.
+      + omega.
+      + break_exists. break_and. subst.
+        exists x0. find_apply_lem_hyp findAtIndex_elim. intuition.
+        break_if.
+        * congruence.
+        * pose proof (leader_sublog_invariant_invariant _ $(eauto)$).
+          unfold leader_sublog_invariant, leader_sublog_host_invariant in *. break_and.
+          eauto.
+  Qed.
+
+  Lemma prevLog_leader_sublog_do_generic_server :
+    raft_net_invariant_do_generic_server prevLog_leader_sublog.
+  Proof.
+    unfold raft_net_invariant_do_generic_server, prevLog_leader_sublog.
+    intros. simpl in *.
+    repeat find_higher_order_rewrite.
+    find_apply_hyp_hyp. break_or_hyp.
+    - break_if; eauto.
+      find_copy_eapply_lem_hyp doGenericServer_type. break_and.
+      find_copy_eapply_lem_hyp doGenericServer_log.
+      repeat find_rewrite.
+      eauto.
+    - find_copy_eapply_lem_hyp doGenericServer_packets.
+      subst. simpl in *. intuition.
+  Qed.
+
+  Lemma prevLog_leader_sublog_state_same_packet_subset :
+    raft_net_invariant_state_same_packet_subset prevLog_leader_sublog.
+  Proof.
+    unfold raft_net_invariant_state_same_packet_subset, prevLog_leader_sublog.
+    intros.
+    find_apply_hyp_hyp.
+    repeat find_reverse_higher_order_rewrite.
+    eauto.
+  Qed.
+
+  Lemma prevLog_leader_sublog_reboot :
+    raft_net_invariant_reboot prevLog_leader_sublog.
+  Proof.
+    unfold raft_net_invariant_reboot, prevLog_leader_sublog, reboot.
+    intros.  subst. simpl in *.
+    repeat find_reverse_higher_order_rewrite.
+
+    match goal with
+    | [ H : context [In _ _], H' : In _ _ |- _ ] =>
+      eapply H with (leader0 := leader) in H'; eauto
+    end.
+    - break_exists_exists. intuition.
+      repeat find_higher_order_rewrite.
+      break_if; subst; simpl in *; auto.
+    - repeat find_higher_order_rewrite.
+      break_if; subst; simpl in *; auto.
+      discriminate.
+    - repeat find_higher_order_rewrite.
+      break_if; subst; simpl in *; auto.
+  Qed.
+
+  Lemma prevLog_leader_sublog_invariant :
+    forall net,
+      raft_intermediate_reachable net ->
+      prevLog_leader_sublog net.
+  Proof.
+    intros.
+    apply raft_net_invariant; auto.
+    - apply prevLog_leader_sublog_init.
+    - apply prevLog_leader_sublog_client_request.
+    - apply prevLog_leader_sublog_timeout.
+    - apply prevLog_leader_sublog_append_entries.
+    - apply prevLog_leader_sublog_append_entries_reply.
+    - apply prevLog_leader_sublog_request_vote.
+    - apply prevLog_leader_sublog_request_vote_reply.
+    - apply prevLog_leader_sublog_do_leader.
+    - apply prevLog_leader_sublog_do_generic_server.
+    - apply prevLog_leader_sublog_state_same_packet_subset.
+    - apply prevLog_leader_sublog_reboot.
+  Qed.
+
   Instance pllsi : prevLog_leader_sublog_interface.
   Proof.
     constructor.
-  Admitted.
+    apply prevLog_leader_sublog_invariant.
+  Qed.
 End PrevLogLeaderSublogProof.
