raft/PrevLogCandidateEntriesTermInterface.v
@@ -1,0 +1,31 @@
+Require Import List.
+Import ListNotations.
+
+Require Import Util.
+Require Import Net.
+
+Require Import Raft.
+Require Import RaftRefinementInterface.
+Require Export CommonDefinitions.
+Require Export RefinementCommonDefinitions.
+
+Section PrevLogCandidateEntriesTermInterface.
+  Context {orig_base_params : BaseParams}.
+  Context {one_node_params : OneNodeParams orig_base_params}.
+  Context {raft_params : RaftParams orig_base_params}.
+
+  Definition prevLog_candidateEntriesTerm (net : network) :=
+    forall p t leaderId prevLogIndex prevLogTerm entries leaderCommit,
+      In p (nwPackets net) ->
+      pBody p = AppendEntries t leaderId prevLogIndex prevLogTerm
+                              entries leaderCommit ->
+      candidateEntriesTerm prevLogTerm (nwState net).
+
+  Class prevLog_candidateEntriesTerm_interface : Prop :=
+    {
+      prevLog_candidateEntriesTerm_invariant :
+        forall net,
+          refined_raft_intermediate_reachable net ->
+          prevLog_candidateEntriesTerm net
+    }.
+End PrevLogCandidateEntriesTermInterface.
